src/OCL_compiler_parser_UML_extended.thy
@@ -45,7 +45,7 @@ header{* Part ... *}
 
 theory  OCL_compiler_parser_UML_extended
 imports OCL_compiler_meta_UML_extended
-        OCL_compiler_parser_init
+        OCL_compiler_parser_oid
 begin
 
 section{* Generation to both Form (setup part) *}
